CP: 1) refined more Ott relations as Coq functions. For example,    a relation 'compute a = b', b should be the output of    this function, because if defined as relations, we    cannot use it in monads, to assign a new value to b.    So we redefined such relations in ssa_lib.ott, and moved    them into ssa_coq_lib.v. I dont know how Ott can solve    this problem.
2) Ott has another bug. If there are multi 'embed blocks'
   in different files, when -merge = true, Ott will merge
   them together, but ignore the dependency from Coq to Ott.
   The grammar homs some datatype to be monads which is defined
   in Coq, so we should define monads in an embed block before
   grammar definitions, but the bug stops it. We temporally
   refined monads as option, they have the same type.

3) defined more monads syntax for imperative programming:
   if-then, if-then-else, if-then-elseif..., for-loop, ...
   with which we can program C++ SSA well-formedness.
   The Coq formalism is more readable, but have no idea
   if it is also easier to prove...
   

git-svn-id: https://webdav.seas.upenn.edu/svn/sol/vol@2341 eef5ea85-cc2e-0410-bd84-0fae1f012da8

src/ssa/monads/Monad.v
@@ -1,19 +1,27 @@
 Require Import Coq.Logic.FunctionalExtensionality.
 Require Import List.
 
-Implicit Type X Y Z W : Set.
+Implicit Type X Y Z W : Type.
 
+Notation monad := option.
+
+Notation munit := Some.
+
+Notation merror := None.
+
+(*
 Inductive monad (X:Type) : Type :=
 | munit : forall (x:X), monad X
 | merror : monad X
 .
 
 Hint Constructors monad.
+*)
 
 Definition mbind (X:Type) (Y:Type) (f:X -> monad Y) (mx:monad X) : monad Y :=
 match mx with
 | munit x => f x
-| merror => merror Y
+| merror => merror
 end.
 
 Definition mif (X:Type) (c:bool) (tclause : monad X) (fclause : monad X) : monad X :=
@@ -29,6 +37,16 @@ match cases with
 | (false, action)::cases' => mswitch _ cases' default_case
 end.
 
+Fixpoint mfor (X:Type) (li:list X) (f:X->monad Prop) : monad Prop :=
+match li with
+| nil => munit True
+| i::li' => 
+  match (f i) with
+  | munit True => mfor _ li' f
+  | _ => merror
+  end
+end.
+
 Notation "'ret' x" := (@munit _ x) (at level 41).
 Notation "x >>= f" := (@mbind _ _ f x) (at level 42, left associativity).
 Notation "e1 >> e2" := (e1 >>= (fun _ => e2)) (at level 42, left associativity).
@@ -36,16 +54,17 @@ Notation "'do' x <- a ; b" := ( a >>= (fun x => b) ) (at level 42, left associat
 Notation "'do' a ; b" := ( a >> b ) (at level 42, left associativity).
 Notation "'do' a 'enddo'" := ( a ) (at level 42, left associativity).
 Notation "'If' b 'then' t 'else' f 'endif'" := (mif _ b t f) (at level 43).
-Notation "'If' b 'then' t 'endif'" := (mif _ b t (munit _ True)) (at level 43).
+Notation "'If' b 'then' t 'endif'" := (mif _ b t (ret True)) (at level 43).
 Notation "'switch' cases 'default' default 'endswitch'" := ( mswitch _ cases default ) (at level 44). 
+Notation "'for' i 'in' li 'do' block 'endfor'" := (mfor _ li (fun i => block)) (at level 44).
 
-Definition mifk (X Y:Set) (c:bool) (tclause : monad X) (fclause : monad X) (con : X -> monad Y) : monad Y :=
+Definition mifk (X Y:Type) (c:bool) (tclause : monad X) (fclause : monad X) (con : X -> monad Y) : monad Y :=
 match c with
 | true => tclause >>= con
 | false => fclause >>= con
 end.
 
-Fixpoint mswitchk (X Y:Set) (cases : list (bool*monad X)) (default_case : monad X) (con : X -> monad Y) : monad Y :=
+Fixpoint mswitchk (X Y:Type) (cases : list (bool*monad X)) (default_case : monad X) (con : X -> monad Y) : monad Y :=
 match cases with
 | nil => default_case >>= con
 | (true, action)::cases' => action >>= con
@@ -129,7 +148,7 @@ Lemma munit_mbind_match : forall X
 Proof.
 intros. transitivity (x >>= @munit X).
 apply mbind_congr; trivial.
-auto with monad.
+unfold mbind. destruct x; auto.
 Qed.
 
 Hint Resolve mbind_congr munit_mbind_match : monad.
@@ -161,19 +180,19 @@ Qed.
 Lemma mmap_mmap : forall X Y Z (f : X -> Y) (g : Y -> Z) (x : monad X),
   (x >>- f) >>- g = x >>- (fun u => g (f u)).
 Proof.
-unfold mmap; monad.
+unfold mmap. unfold mbind; monad. destruct x; auto.
 Qed.
 
 Lemma mmap_mbind : forall X Y Z (f : X -> Y) (g : Y -> monad Z) (x : monad X),
   x >>- f >>= g = x >>= (fun u => g (f u)).
 Proof.
-unfold mmap; monad.
+unfold mmap. unfold mbind; monad. destruct x; auto.
 Qed.
 
 Lemma mbind_mmap : forall X Y Z (f : X -> monad Y) (g : Y -> Z) (x : monad X),
   x >>= f >>- g = x >>= (fun u => f u >>- g).
 Proof.
-unfold mmap; monad.
+unfold mmap. unfold mbind; monad. destruct x; auto.
 Qed.
 
 Hint Rewrite mmap_munit mmap_mmap mmap_mbind mbind_mmap : monad.
@@ -181,7 +200,7 @@ Hint Rewrite mmap_munit mmap_mmap mmap_mbind mbind_mmap : monad.
 Lemma mjoin_mjoin : forall X (x : monad (monad (monad X))),
   mjoin X (mjoin (monad X) x) = mjoin X (x >>- (mjoin X)).
 Proof.
-unfold mjoin; monad.
+unfold mjoin. unfold mbind; monad. destruct x; auto.
 Qed.
 
 Lemma mjoin_munit : forall X (x : monad X),
@@ -191,9 +210,9 @@ unfold mjoin; monad.
 Qed.
 
 Lemma munit_mjoin : forall X (x : monad X),
-  mjoin X (x >>- munit X) = x.
+  mjoin X (x >>- @munit X) = x.
 Proof.
-unfold mjoin; monad.
+unfold mjoin. unfold mbind; monad. destruct x; auto.
 Qed.
 
 Lemma mjoin_mmap : forall X Y (f : X -> monad Y) (x : monad X),
